libs/ffi/mitlsffi.h
@@ -86,7 +86,7 @@ extern int MITLS_CALLCONV FFI_mitls_configure_cipher_suites(/* in */ mitls_state
 extern int MITLS_CALLCONV FFI_mitls_configure_signature_algorithms(/* in */ mitls_state *state, const char * sa);
 extern int MITLS_CALLCONV FFI_mitls_configure_named_groups(/* in */ mitls_state *state, const char * ng);
 extern int MITLS_CALLCONV FFI_mitls_configure_alpn(/* in */ mitls_state *state, const char *apl);
-extern int MITLS_CALLCONV FFI_mitls_configure_early_data(/* in */ mitls_state *state, int enable_early_data);
+extern int MITLS_CALLCONV FFI_mitls_configure_early_data(/* in */ mitls_state *state, uint32_t max_early_data);
 extern int MITLS_CALLCONV FFI_mitls_configure_ticket_callback(mitls_state *state, void *cb_state, pfn_FFI_ticket_cb ticket_cb);
 extern int MITLS_CALLCONV FFI_mitls_configure_cert_callbacks(mitls_state *state, void *cb_state, mitls_cert_cb *cert_cb);
 
